src/program_proof/ctrexample/client.v
@@ -1,0 +1,89 @@
+From Perennial.goose_lang Require Import prelude.
+From Perennial.goose_lang Require Export ffi.grove_prelude.
+From Perennial.program_proof Require Import proof_prelude.
+From Perennial.goose_lang Require Export ffi.grove_filesys_axioms.
+From Perennial.program_proof.ctrexample Require Import interface.
+From Perennial.program_proof Require Import marshal_proof.
+From Goose.github_com.mit_pdos.gokv.ctrexample Require Import client.
+From Perennial.program_proof.memkv Require Import rpc_proof.
+From Perennial.program_proof.ctrexample Require Import wpc_proofmode.
+
+Section client_proof.
+
+Context `{!heapGS Σ}.
+Context `{!filesysG Σ}.
+Context `{!inG Σ mono_natUR}.
+Context `{!rpcregG Σ}.
+
+Lemma wpc_ClientMain γurpc_gn γ :
+  is_CtrServer_urpc γurpc_gn γ -∗
+    counter_lb γ 0 -∗
+    WP main #()
+  {{
+      v, True
+  }}.
+Proof.
+  iIntros "#Hsrv #Hlb".
+  wp_lam.
+  wp_pures.
+  wp_apply (wp_MakeRPCClient).
+  iIntros (cl_ptr) "Hcl".
+  wp_pures.
+  wp_apply (wp_ref_to).
+  { eauto. }
+  iIntros (localBound_ptr) "HlocalBound".
+  wp_pures.
+
+  iAssert (∃ x, counter_lb γ x ∗ localBound_ptr ↦[uint64T] #(U64 x))%I with "[HlocalBound Hlb]" as "HH".
+  {
+    iExists 0%nat. iFrame "#∗".
+  }
+  wp_forBreak.
+  wp_pures.
+
+  iClear "Hlb".
+  iDestruct "HH" as (localBound) "[#Hlb HlocalBound]".
+
+  wp_apply (wp_ref_of_zero).
+  { done. }
+  iIntros (rep) "Hrep".
+  wp_pures.
+  wp_apply (wp_NewSlice _ _ byteT).
+  iIntros (empty_req) "Hempty_sl".
+
+  wp_apply (wp_RPCClient__Call with "[$Hcl $Hrep $Hempty_sl]").
+  {
+    iDestruct "Hsrv" as "[$ _]".
+    instantiate (1:=(λ l, ∃ (x:nat), ⌜has_encoding l [EncUInt64 (U64 x)] ∧ x ≤ localBound⌝)%I).
+    iModIntro.
+    iModIntro.
+    simpl.
+    iIntros (x) "Hctr".
+    unfold counter_own.
+    rewrite mono_nat_auth_lb_op.
+    iDestruct (own_op with "Hctr") as "[Hctr #Hlb2]".
+    iDestruct (own_update with "Hctr") as ">$".
+    { apply mono_nat_update. word. }
+    iModIntro.
+    iIntros.
+    iExists x.
+    unfold counter_lb.
+    iFrame "#".
+    admit.
+  }
+  iIntros (err) "(Hcl & Hreq & Hrep)".
+  destruct err.
+  {
+    wp_pures.
+    wp_if_destruct.
+    {
+      admit.
+    }
+    admit.
+  }
+  iNamed "Hrep".
+  iDestruct "Hrep" as "(Hrep & Hrep_sl & HPost)".
+  iDestruct "HPost" as (x) ">[%HencPost #Hlb2]".
+  wp_pures.
+
+End client_proof.
